test/hand_crafted/functions.py
@@ -1,0 +1,30 @@
+def top_level():
+    """Tests for calling/defining functions
+    """
+    
+    def test_function_def_with_no_params():
+        return 1
+    
+    def test_function_def_with_params(x,y,z):
+        return x, y, z
+    
+    def test_recursive(x):
+        if x <= 0:
+            return 0    
+        return x + test_recursive(x-1)
+        
+    def test_function_to_be_called():
+        return 1
+    
+    def test_caller_function():
+        return test_function_to_be_called()
+    
+    
+    result = [
+        test_function_def_with_no_params(),
+        test_function_def_with_params(1,2,3),
+        test_recursive(5),
+        test_caller_function()
+    ]
+    
+    return result
