test/test.py
@@ -1,8 +1,19 @@
-def top_level():
-    def test():
-        return 7
+# def top_level():
+#     def test():
+#         return 5
     
-    def test2():
-        return 3
+#     def test2():
+#         return test()
     
-    return (test() * test2())
+#     return (test2())
+
+# def test(x):
+#     if x == 0:
+#         return 1
+#     test(x-1)
+    
+# test(5)
+
+x = [1,2,3,4,5,6]
+y = x[5:-1:-1]
+print(y)
