src/test/Test.fst
@@ -7,66 +7,84 @@ open Utils
 open PyBuiltinObjects
 (* ---------------- *)
 
-let bc_0x7f2c2b61cdf0 = CODE [
+let bc_0x7fec7faa6a80 = CODE [
   LOAD_CONST 1;
   LOAD_CONST 2;
   MAKE_FUNCTION 0;
   STORE_FAST 0;
-  LOAD_CONST 3;
-  LOAD_CONST 4;
-  MAKE_FUNCTION 0;
-  STORE_FAST 1;
-  LOAD_CONST 5;
-  LOAD_CONST 6;
-  MAKE_FUNCTION 0;
-  STORE_FAST 2;
   LOAD_FAST 0;
   CALL_FUNCTION 0;
+  BUILD_LIST 1;
+  STORE_FAST 1;
   LOAD_FAST 1;
-  CALL_FUNCTION 0;
-  LOAD_FAST 2;
-  CALL_FUNCTION 0;
-  BUILD_LIST 3;
-  STORE_FAST 3;
-  LOAD_FAST 3;
   RETURN_VALUE ;
 ]
 
-let bc_0x7f2c2b61cd40 = CODE [
+let bc_0x7fec7faa69d0 = CODE [
   LOAD_CONST 1;
-  STORE_FAST 0;
   LOAD_CONST 2;
-  STORE_FAST 1;
-  LOAD_CONST 1;
-  STORE_FAST 2;
-  LOAD_CONST 2;
-  STORE_FAST 3;
-  LOAD_CONST 2;
-  STORE_FAST 4;
-  LOAD_CONST 1;
-  STORE_FAST 5;
-  BUILD_LIST 0;
-  UNARY_NOT ;
-  STORE_FAST 6;
-  LOAD_CONST 3;
-  BUILD_LIST 1;
-  UNARY_NOT ;
-  STORE_FAST 7;
-  LOAD_CONST 1;
-  STORE_FAST 8;
-  LOAD_CONST 2;
-  STORE_FAST 9;
-  BUILD_MAP 0;
-  UNARY_NOT ;
-  STORE_FAST 10;
   LOAD_CONST 3;
   LOAD_CONST 4;
-  BUILD_MAP 1;
-  UNARY_NOT ;
-  STORE_FAST 11;
-  LOAD_CONST 1;
-  STORE_FAST 12;
+  LOAD_CONST 5;
+  LOAD_CONST 6;
+  LOAD_CONST 7;
+  LOAD_CONST 8;
+  LOAD_CONST 9;
+  BUILD_LIST 9;
+  STORE_FAST 0;
   LOAD_FAST 0;
+  LOAD_CONST 0;
+  LOAD_CONST 0;
+  BUILD_SLICE 2;
+  BINARY_SUBSCR ;
+  STORE_FAST 1;
+  LOAD_FAST 0;
+  LOAD_CONST 0;
+  LOAD_CONST 0;
+  LOAD_CONST 10;
+  BUILD_SLICE 3;
+  BINARY_SUBSCR ;
+  STORE_FAST 2;
+  LOAD_FAST 0;
+  LOAD_CONST 0;
+  LOAD_CONST 0;
+  LOAD_CONST 2;
+  BUILD_SLICE 3;
+  BINARY_SUBSCR ;
+  STORE_FAST 3;
+  LOAD_FAST 0;
+  LOAD_CONST 0;
+  LOAD_CONST 0;
+  LOAD_CONST 11;
+  BUILD_SLICE 3;
+  BINARY_SUBSCR ;
+  STORE_FAST 4;
+  LOAD_FAST 0;
+  LOAD_CONST 12;
+  LOAD_CONST 13;
+  BUILD_SLICE 2;
+  BINARY_SUBSCR ;
+  STORE_FAST 5;
+  LOAD_FAST 0;
+  LOAD_CONST 14;
+  LOAD_CONST 0;
+  LOAD_CONST 10;
+  BUILD_SLICE 3;
+  BINARY_SUBSCR ;
+  STORE_FAST 6;
+  LOAD_FAST 0;
+  LOAD_CONST 5;
+  LOAD_CONST 1;
+  BUILD_SLICE 2;
+  BINARY_SUBSCR ;
+  STORE_FAST 7;
+  LOAD_FAST 0;
+  LOAD_CONST 1;
+  LOAD_CONST 5;
+  LOAD_CONST 10;
+  BUILD_SLICE 3;
+  BINARY_SUBSCR ;
+  STORE_FAST 8;
   LOAD_FAST 1;
   LOAD_FAST 2;
   LOAD_FAST 3;
@@ -75,166 +93,71 @@ let bc_0x7f2c2b61cd40 = CODE [
   LOAD_FAST 6;
   LOAD_FAST 7;
   LOAD_FAST 8;
-  LOAD_FAST 9;
-  LOAD_FAST 10;
-  LOAD_FAST 11;
-  LOAD_FAST 12;
-  BUILD_TUPLE 13;
+  BUILD_TUPLE 8;
   RETURN_VALUE ;
 ]
 
-let consts_0x7f2c2b61cd40 = [
+let consts_0x7fec7faa69d0 = [
   PYTYP(createNone());
-  PYTYP(createBool true);
-  PYTYP(createBool false);
   PYTYP(createInt 1);
   PYTYP(createInt 2);
-]
-
-let varnames_0x7f2c2b61cd40 = [
-  "x11";
-  "x12";
-  "x21";
-  "x22";
-  "x31";
-  "x32";
-  "x41";
-  "x42";
-  "x51";
-  "x52";
-  "x61";
-  "x62";
-  "x7";
-]
-
-let names_0x7f2c2b61cd40 = [
-]
-
-let co_0x7f2c2b61cd40 = {
-  co_code = bc_0x7f2c2b61cd40;
-  co_consts = consts_0x7f2c2b61cd40;
-  co_varnames = varnames_0x7f2c2b61cd40;
-  co_names = names_0x7f2c2b61cd40
-}
-
-let bc_0x7f2c2b61cc90 = CODE [
-  LOAD_CONST 1;
-  STORE_FAST 0;
-  LOAD_FAST 0;
-  LOAD_CONST 2;
-  INPLACE_SUBTRACT ;
-  STORE_FAST 0;
-  LOAD_FAST 0;
-  RETURN_VALUE ;
-]
-
-let consts_0x7f2c2b61cc90 = [
-  PYTYP(createNone());
-  PYTYP(createInt 2);
-  PYTYP(createInt 1);
-]
-
-let varnames_0x7f2c2b61cc90 = [
-  "x";
-]
-
-let names_0x7f2c2b61cc90 = [
-]
-
-let co_0x7f2c2b61cc90 = {
-  co_code = bc_0x7f2c2b61cc90;
-  co_consts = consts_0x7f2c2b61cc90;
-  co_varnames = varnames_0x7f2c2b61cc90;
-  co_names = names_0x7f2c2b61cc90
-}
-
-let bc_0x7f2c2b61cbe0 = CODE [
-  LOAD_CONST 1;
-  STORE_FAST 0;
-  LOAD_CONST 2;
-  BUILD_LIST 1;
-  STORE_FAST 1;
-  LOAD_CONST 2;
-  STORE_FAST 2;
-  LOAD_CONST 3;
-  STORE_FAST 3;
-  LOAD_FAST 0;
-  LOAD_CONST 2;
-  INPLACE_ADD ;
-  STORE_FAST 0;
-  LOAD_FAST 1;
-  LOAD_CONST 4;
-  BUILD_LIST 1;
-  INPLACE_ADD ;
-  STORE_FAST 1;
-  LOAD_FAST 2;
-  LOAD_CONST 4;
-  INPLACE_ADD ;
-  STORE_FAST 2;
-  LOAD_FAST 3;
-  LOAD_CONST 5;
-  INPLACE_ADD ;
-  STORE_FAST 3;
-  LOAD_FAST 0;
-  LOAD_FAST 1;
-  LOAD_FAST 2;
-  LOAD_FAST 3;
-  BUILD_TUPLE 4;
-  RETURN_VALUE ;
-]
-
-let consts_0x7f2c2b61cbe0 = [
-  PYTYP(createNone());
+  PYTYP(createInt 3);
+  PYTYP(createInt 4);
+  PYTYP(createInt 5);
+  PYTYP(createInt 6);
+  PYTYP(createInt 7);
+  PYTYP(createInt 8);
+  PYTYP(createInt 9);
+  PYTYP(createInt (-1));
+  PYTYP(createInt (-2));
   PYTYP(createInt 0);
-  PYTYP(createInt 1);
-  PYTYP(createString "");
-  PYTYP(createInt 2);
-  PYTYP(createString "1");
+  PYTYP(createInt 15);
+  PYTYP(createInt (-10));
 ]
 
-let varnames_0x7f2c2b61cbe0 = [
+let varnames_0x7fec7faa69d0 = [
+  "l2";
   "x1";
   "x2";
   "x3";
   "x4";
+  "x5";
+  "x6";
+  "x7";
+  "x8";
 ]
 
-let names_0x7f2c2b61cbe0 = [
+let names_0x7fec7faa69d0 = [
 ]
 
-let co_0x7f2c2b61cbe0 = {
-  co_code = bc_0x7f2c2b61cbe0;
-  co_consts = consts_0x7f2c2b61cbe0;
-  co_varnames = varnames_0x7f2c2b61cbe0;
-  co_names = names_0x7f2c2b61cbe0
+let co_0x7fec7faa69d0 = {
+  co_code = bc_0x7fec7faa69d0;
+  co_consts = consts_0x7fec7faa69d0;
+  co_varnames = varnames_0x7fec7faa69d0;
+  co_names = names_0x7fec7faa69d0
 }
 
-let consts_0x7f2c2b61cdf0 = [
-  PYTYP(createNone());
-  CODEOBJECT(co_0x7f2c2b61cbe0);
-  PYTYP(createString "top_level.<locals>.test_UNARY_POSITIVE");
-  CODEOBJECT(co_0x7f2c2b61cc90);
-  PYTYP(createString "top_level.<locals>.test_UNARY_NEGATIVE");
-  CODEOBJECT(co_0x7f2c2b61cd40);
-  PYTYP(createString "top_level.<locals>.test_UNARY_NOT");
+let consts_0x7fec7faa6a80 = [
+  PYTYP(createString "Test cases for Binary operations
+    ");
+  CODEOBJECT(co_0x7fec7faa69d0);
+  PYTYP(createString "top_level.<locals>.test_BINARY_SUBSCR_SLICES");
 ]
 
-let varnames_0x7f2c2b61cdf0 = [
-  "test_UNARY_POSITIVE";
-  "test_UNARY_NEGATIVE";
-  "test_UNARY_NOT";
+let varnames_0x7fec7faa6a80 = [
+  "test_BINARY_SUBSCR_SLICES";
   "result";
 ]
 
-let names_0x7f2c2b61cdf0 = [
+let names_0x7fec7faa6a80 = [
 ]
 
-let co_0x7f2c2b61cdf0 = {
-  co_code = bc_0x7f2c2b61cdf0;
-  co_consts = consts_0x7f2c2b61cdf0;
-  co_varnames = varnames_0x7f2c2b61cdf0;
-  co_names = names_0x7f2c2b61cdf0
+let co_0x7fec7faa6a80 = {
+  co_code = bc_0x7fec7faa6a80;
+  co_consts = consts_0x7fec7faa6a80;
+  co_varnames = varnames_0x7fec7faa6a80;
+  co_names = names_0x7fec7faa6a80
 }
 
-let virt_m, res = runCode_returnVM co_0x7f2c2b61cdf0
+let virt_m, res = runCode_returnVM co_0x7fec7faa6a80
 let print_program_state = IO.print_string (print_program_state virt_m res)
